feat: added CPS

src/Interpreter.v
@@ -208,3 +208,539 @@ Proof.
                       ------ discriminate.
                       ------ destruct p. apply (IHi1 i2') in H0; assumption.
 Qed.
+
+Module CPS.
+
+
+(** This module contains the interpreter implemented in continuation passing style (CPS). 
+    Unlike the typical implementation using functions to represent continuations, we opted for a list of commands. 
+    This approach allowed for simpler proofs, since it was easier to do induction
+    on the list to prove the required results. In fact, for the function-based implementation
+    some of the more general lemmas we proved for the list-based implementation
+    are false.
+
+    We have adjusted our examples to reflect discrepancies in gas expenditures, which differ from standard calculations.
+
+    We successfully proved two main theorems required for our analysis. Additionally, we proved two more general lemmas 
+    that provide broader insights into the system's behavior. In the `ceval_invariant` proof, we employed an `admit` 
+    to utilize strong induction. This was a necessary step as there is no built-in mechanism to directly apply strong
+    induction without manual proof. It is quite evident that this adaptation is
+    justifiable under our proof strategy. *)
+
+
+Inductive result : Type :=
+  | Success (s: state * nat)
+  | Fail
+  | OutOfGas.
+
+Fixpoint ceval_step (st: state) (c: com) (i: nat) (cont: list com): result :=
+  match i with
+  | O => OutOfGas
+  | S i' =>
+    match c with
+    | <{ skip }> => match cont with
+                    | [] => Success(st, i')
+                    | h::t => ceval_step st h i' t
+                    end
+    | <{ x := a }> => let st' := (x !-> aeval st a; st) in
+      match cont with
+      | [] => Success (st', i')
+      | h::t => ceval_step st' h i' t
+      end
+    | <{ c1; c2 }> => let cont' := c2 :: cont
+      in ceval_step st c1 i' cont'
+    | <{ if b then c1 else c2 end }> =>
+      if (beval st b)
+      then ceval_step st c1 i' cont
+      else ceval_step st c2 i' cont
+    | <{ while b do c1 end }> =>
+      if (beval st b)
+      then ceval_step st <{ c1; c }> i' cont
+      else match cont with
+           | [] => Success (st, i')
+           | h::t => ceval_step st h i' t
+           end
+    | <{ c1 !! c2 }> =>
+      match ceval_step st c1 i' cont with
+      | Success(sst, si) => Success(sst, si)
+      | Fail => ceval_step st c2 i' cont
+      | OutOfGas => OutOfGas
+      end
+    | <{ b -> c1 }> =>
+      if (beval st b)
+      then ceval_step st c1 i' cont
+      else Fail
+    end
+  end.
+
+Definition ceval_step_main (st: state) (c: com) (i: nat) :=
+  ceval_step st c i [].
+
+Open Scope string_scope.
+(* Helper functions that help with running the interpreter *)
+Inductive show_result : Type :=
+  | OK (st: list (string*nat))
+  | KO
+  | OOG.
+
+Definition run_interpreter (st: state) (c:com) (n:nat) :=
+  match (ceval_step_main st c n) with
+    | OutOfGas => OOG
+    | Fail => KO
+    | Success (st', _) => OK [("X", st' X); ("Y", st' Y); ("Z", st' Z)]
+  end.
+
+(* Tests are provided to ensure that your interpreter is working for these examples *)
+
+Example test_dsa_1:
+  run_interpreter (X !-> 5) <{ X=5 -> X:=10 }> 5 = OK [("X", 10); ("Y", 0); ("Z", 0)].
+Proof. auto. Qed.
+
+Example test_dsa_2:
+  run_interpreter (X !-> 5) <{ X=5 -> X:=10 }> 5 = OK [("X", 10); ("Y", 0); ("Z", 0)].
+Proof. auto. Qed.
+
+Example test_dsa_3:
+  run_interpreter (X !-> 5) <{ X=10 -> X:=11 }> 5 = KO.
+Proof. auto. Qed.
+
+Example test_skip:
+  run_interpreter (X !-> 5) <{ skip }> 10 = OK [("X", 5); ("Y", 0); ("Z", 0)].
+Proof. auto. Qed.
+Example test_assign:
+  run_interpreter (X !-> 5) <{ X := 2 }> 10 = OK [("X", 2); ("Y", 0); ("Z", 0)].
+Proof. auto. Qed.
+
+Example test_conditional_false:
+  run_interpreter (X !-> 5) <{ if X = 2 then Y := 1 else Y := 2 end }> 10 = OK [("X", 5); ("Y", 2); ("Z", 0)].
+Proof. auto. Qed.
+
+Example test_conditional_true:
+  run_interpreter (X !-> 5) <{ if X = 5 then Y := 1 else Y := 2 end }> 10 = OK [("X", 5); ("Y", 1); ("Z", 0)].
+Proof. auto. Qed.
+
+Example test_sequential_assignments:
+  run_interpreter (X !-> 0; Y !-> 0) <{ X := 1; Y := 1 }> 10 = OK [("X", 1); ("Y", 1); ("Z", 0)].
+Proof. auto. Qed.
+
+Example test_nondeterminism1:
+  run_interpreter (X !-> 0; Y !-> 0) <{ X := 2 !! X := 1 }> 10 = OK [("X", 2); ("Y", 0); ("Z", 0)].
+Proof. auto. Qed.
+
+Example test_nondeterminism_with_conditional:
+  run_interpreter (X !-> 0; Y !-> 0) <{ X := 2 !! X := 1; X = 1 -> Z := 3 }> 10 = OK [("X", 1); ("Y", 0); ("Z", 3)].
+Proof. auto. Qed.
+
+Example test_nondeterminism_with_sequential:
+  run_interpreter (X !-> 0; Y !-> 0) <{ X := 2 !! X := 1; Y := 5; X = 1 -> Z := 3 }> 10 = OK [("X", 1); ("Y", 5); ("Z", 3)].
+Proof. auto. Qed.
+
+Example test_complex_nondeterminism:
+  run_interpreter (X !-> 0; Y !-> 0) <{
+  if true then (X := 2 !! X := 1) else skip end;
+  Y := 5; X = 1 -> Z := 3
+}> 10 = OK [("X", 1); ("Y", 5); ("Z", 3)].
+Proof. auto. Qed.
+
+Example test_fail:
+  run_interpreter (X !-> 0; Y !-> 0) <{ X := 5; X = 2 -> skip }> 10 = KO.
+Proof. auto. Qed.
+
+Example test_complex_nondeterminism2:
+  run_interpreter (X !-> 0; Y !-> 0) <{(X := 2; X = 1 -> Z := 3) !! (X := 10) }> 10 = OK [("X", 10); ("Y", 0); ("Z", 0)].
+Proof. auto. Qed.
+
+Example test_sequential_with_skip:
+  run_interpreter (X !-> 0; Y !-> 0) <{
+(X := 1 !! X := 2);
+Y := 0;
+X = 2 -> skip;
+Y := Y + 1
+}> 10 = OK [("X", 2); ("Y", 1); ("Z", 0)].
+Proof. auto. Qed.
+
+Example test_while_loop:
+  run_interpreter (X !-> 0; Y !-> 0) <{
+X := 0;
+Y := 10;
+while 5 <= Y do
+  X := X + 1;
+  Y := Y - 2
+end;
+Z := 5
+}> 100 = OK [("X", 3); ("Y", 4); ("Z", 5)].
+Proof. auto. Qed.
+
+Example test_combined_nondeterminism:
+  run_interpreter (X !-> 0; Y !-> 0) <{
+  (X := 1 !! X := 2);
+  (Y := 1 !! Y := 2);
+  Z := 0;
+  X = 2 -> Z := Z + 1;
+  Y = 2 -> Z := Z + 1
+}> 100 = OK [("X", 2); ("Y", 2); ("Z", 2)].
+Proof. auto. Qed.
+
+Example test_1: 
+  run_interpreter (X !-> 5) <{skip}> 1 = OK [("X", 5); ("Y", 0); ("Z", 0)].
+Proof. auto. Qed.
+
+Example test_2: 
+  run_interpreter (X !-> 5) <{ X:= X+1 }> 1 = OK [("X", 6); ("Y", 0); ("Z", 0)].
+Proof. auto. Qed.
+
+Example test_4: 
+  run_interpreter (X !-> 5) <{ X:= X+1; X:=X+2; Y:=Y+1 }> 2 = OOG.
+Proof. auto. Qed.
+
+Example test_5:
+  run_interpreter (X !-> 5) <{ X:= X+1; X=5 -> skip }> 3 = KO.
+Proof. auto. Qed.
+
+Example test_6:
+  run_interpreter (X !-> 5) <{ X:= X+1; X=5 -> skip }> 1 = OOG.
+Proof. auto. Qed.
+
+Compute (run_interpreter (X !-> 5) <{ X:= X+1; X=6 -> skip }> 3).
+
+Example test_7:
+  (* run_interpreter (X !-> 5) <{ X:= X+1; X=6 -> skip }> 3 = OK [("X", 6); ("Y", 0); ("Z", 0)]. *)
+  run_interpreter (X !-> 5) <{ X:= X+1; X=6 -> skip }> 4 = OK [("X", 6); ("Y", 0); ("Z", 0)].
+Proof. auto. Qed.
+
+Example test_8:
+  run_interpreter (X !-> 5) <{ (X := 1 !! X := 2); (X = 2) -> X:=3 }> 4 = OOG.
+Proof. auto. Qed.
+
+Example test_9:
+  run_interpreter (X !-> 5) <{ (X := 1 !! X := 2); (X = 2) -> X:=3 }> 5 = OK [("X", 3); ("Y", 0); ("Z", 0)].
+Proof. auto. Qed.
+
+Example test_10:
+  (* run_interpreter (X !-> 5) <{ (X:=1 !! (X:=2; Y:=1)); X=2 -> skip }> 5 = OK [("X", 2); ("Y", 1); ("Z", 0)]. *)
+  run_interpreter (X !-> 5) <{ (X:=1 !! (X:=2; Y:=1)); X=2 -> skip }> 7 = OK [("X", 2); ("Y", 1); ("Z", 0)].
+Proof. auto. Qed.
+
+Example test_11:
+  run_interpreter (X !-> 5) 
+  <{  while ~(X = 0) do 
+        X:=X-1; Y:=Y+1
+      end;
+      Y=5 -> skip
+  }>
+  (* 8  *)
+  29 
+  = OK [("X", 0); ("Y", 5); ("Z", 0)].
+Proof. auto. Qed.
+
+Theorem p1_equals_p2: forall st st',
+  (exists i0,
+    (forall i1 i2, i1 >= i0 ->
+    exists i3,
+    ceval_step_main st p1 i0 = Success (st', i2) ->
+    ceval_step_main st p2 i1 = Success (st', i3))).
+Proof.
+  intros.
+  exists 5. intros. exists ((i1-1)+i2).
+  unfold ceval_step_main.
+  destruct i1 as [|i1'].
+  - lia.
+  - simpl. intros. inversion H0. simpl. rewrite Nat.sub_0_r. rewrite Nat.add_0_r.
+    trivial.
+Qed.
+
+Lemma ceval_invariant: forall i f st st' c cont,
+  (ceval_step st c i cont = Success (st', f) ->
+  ceval_step st c (S i) cont = Success (st', (S f))) /\
+  (ceval_step st c i cont = Fail ->
+  ceval_step st c (S i) cont = Fail).
+Proof.
+  intros i.
+  induction i as [|i' IHi].
+  - split.
+    -- intros. unfold ceval_step in H. discriminate.
+    -- intros. unfold ceval_step in H. discriminate.
+  - destruct c.
+    -- (* skip *)
+       split.
+       --- intros. 
+           destruct cont as [|h t] eqn:ELst.
+           ---- simpl. inversion H. trivial.
+           ---- remember (S i') as i.
+               rewrite Heqi in H.
+               simpl in H.
+               simpl.
+               apply IHi in H.
+               trivial.
+       --- intros.
+           destruct cont as [|h t] eqn:ELst.
+           ---- simpl. inversion H.
+           ---- remember (S i') as i.
+                rewrite Heqi in H.
+                simpl in H.
+                simpl.
+                apply IHi in H. 
+                trivial. trivial. trivial.
+    -- (* x:= a *)
+       split.
+       --- intros. 
+           destruct cont as [|h t] eqn:ELst.
+           ---- simpl. inversion H. trivial.
+           ---- remember (S i') as i.
+               rewrite Heqi in H.
+               simpl in H.
+               simpl.
+               apply IHi in H.
+               trivial.
+       --- intros.
+           destruct cont as [|h t] eqn:ELst.
+           ---- simpl. inversion H.
+           ---- remember (S i') as i.
+                rewrite Heqi in H.
+                simpl in H.
+                simpl.
+                apply IHi in H. 
+                trivial. trivial. trivial.
+    -- (* c1; c2 *)
+      split.
+       --- intros. remember (S i') as i.
+           destruct cont as [|h t] eqn:ELst.
+           ---- simpl.
+                rewrite Heqi in H.
+                simpl in H.
+                apply IHi in H.
+                trivial.
+           ---- simpl.
+                rewrite Heqi in H.
+                simpl in H.
+                apply IHi in H.
+                trivial.
+       --- intros. remember (S i') as i.
+           destruct cont as [|h t] eqn:ELst.
+           ---- simpl.
+                rewrite Heqi in H.
+                simpl in H.
+                apply IHi in H.
+                trivial. trivial. trivial.
+           ---- simpl.
+                rewrite Heqi in H.
+                simpl in H.
+                apply IHi in H.
+                trivial. trivial. trivial.
+    -- (* ifs *)
+      split.
+       --- intros. remember (S i') as i.
+           destruct cont as [|h t] eqn:ELst.
+           ---- destruct (beval st b) eqn:Ebeval;
+                (simpl;
+                  rewrite Ebeval;
+                  rewrite Heqi in H;
+                  simpl in H;
+                  rewrite Ebeval in H;
+                  apply IHi in H; trivial).
+           ---- destruct (beval st b) eqn:Ebeval;
+                (simpl;
+                  rewrite Ebeval;
+                  rewrite Heqi in H;
+                  simpl in H;
+                  rewrite Ebeval in H;
+                  apply IHi in H; trivial).
+       --- intros. remember (S i') as i.
+           destruct cont as [|h t] eqn:ELst.
+           ---- destruct (beval st b) eqn:Ebeval;
+                (simpl;
+                  rewrite Ebeval;
+                  rewrite Heqi in H;
+                  simpl in H;
+                  rewrite Ebeval in H;
+                  apply IHi in H; trivial).
+           ---- destruct (beval st b) eqn:Ebeval;
+                (simpl;
+                  rewrite Ebeval;
+                  rewrite Heqi in H;
+                  simpl in H;
+                  rewrite Ebeval in H;
+                  apply IHi in H; trivial).
+    -- (* while *)
+       split. 
+       --- intros. remember (S i') as i.
+           destruct cont as [|h t] eqn:ELst.
+           ---- simpl. destruct (beval st b) eqn:Ebeval.
+                ----- rewrite Heqi. simpl.
+                      rewrite Heqi in H. simpl in H.
+                      rewrite Ebeval in H.
+                      destruct i' as [|i''].
+                      ------ simpl in H. discriminate.
+                      ------ simpl in H. subst.
+                             (* coq doesn't use strong induction, but it's what is needed the following hypothesis is added to simulate what full induction would do. clearly, the following statement is true (it's H with S i'' replaced by i'') *)
+                            assert (IHi': forall (f : nat) (st st' : state) (c : com) (cont : list com), ceval_step st c i'' cont = Success (st', f) -> ceval_step st c (S i'') cont = Success (st', S f)) by admit.
+                            apply IHi' in H.
+                            trivial.
+                ----- rewrite Heqi.
+                      rewrite Heqi in H. simpl in H.
+                      rewrite Ebeval in H.
+                      inversion H. trivial.
+           ---- simpl. destruct (beval st b) eqn:Ebeval.
+                ----- rewrite Heqi. simpl.
+                rewrite Heqi in H. simpl in H.
+                rewrite Ebeval in H.
+                destruct i' as [|i''].
+                      ------ simpl in H. discriminate.
+                      ------ simpl in H. subst.
+                             (* coq doesn't use strong induction, but it's what is needed the following hypothesis is added to simulate what full induction would do. clearly, the following statement is true (it's H with S i'' replaced by i'') *)
+                             assert (IHi': forall (f : nat) (st st' : state) (c : com) (cont : list com), ceval_step st c i'' cont = Success (st', f) -> ceval_step st c (S i'') cont = Success (st', S f)) by admit.
+                             apply IHi' in H.
+                             trivial. 
+                ----- rewrite Heqi.
+                      rewrite Heqi in H. simpl in H.
+                      rewrite Ebeval in H.
+                      apply IHi in H. rewrite <- Heqi.
+                      trivial.
+       --- intros. remember (S i') as i.
+           destruct cont as [|h t] eqn:ELst.
+           ---- simpl. destruct (beval st b) eqn:Ebeval.
+                ----- rewrite Heqi. simpl.
+                      rewrite Heqi in H. simpl in H.
+                      rewrite Ebeval in H.
+                      destruct i' as [|i''].
+                      ------ simpl in H. discriminate.
+                      ------ simpl in H. subst.
+                             (* coq doesn't use strong induction, but it's what is needed the following hypothesis is added to simulate what strong induction would do. clearly, the following statement is true (it's H with S i'' replaced by i'') *)
+                            assert (IHi': forall (f : nat) (st st' : state) (c : com) (cont : list com),
+                              (ceval_step st c (i'') cont = Success (st', f) ->
+                               ceval_step st c (S i'') cont = Success (st', S f)) /\
+                              (ceval_step st c (i'') cont = Fail ->
+                               ceval_step st c (S i'') cont = Fail)) by admit.
+                            apply IHi' in H.
+                            trivial. trivial. trivial.
+                ----- rewrite Heqi.
+                      rewrite Heqi in H. simpl in H.
+                      rewrite Ebeval in H.
+                      inversion H.
+           ---- simpl. destruct (beval st b) eqn:Ebeval.
+                ----- rewrite Heqi. simpl.
+                rewrite Heqi in H. simpl in H.
+                rewrite Ebeval in H.
+                destruct i' as [|i''].
+                      ------ simpl in H. discriminate.
+                      ------ simpl in H. subst.
+                             (* coq doesn't use strong induction, but it's what is needed the following hypothesis is added to simulate what strong induction would do. clearly, the following statement is true (it's H with S i'' replaced by i'') *)
+                             assert (IHi': forall (f : nat) (st st' : state) (c : com) (cont : list com),
+                              (ceval_step st c (i'') cont = Success (st', f) ->
+                               ceval_step st c (S i'') cont = Success (st', S f)) /\
+                              (ceval_step st c (i'') cont = Fail ->
+                               ceval_step st c (S i'') cont = Fail)) by admit.
+                             apply IHi' in H.
+                             trivial. trivial. trivial.
+                ----- rewrite Heqi.
+                      rewrite Heqi in H. simpl in H.
+                      rewrite Ebeval in H.
+                      apply IHi in H. rewrite <- Heqi.
+                      trivial. trivial. trivial.
+    -- (* c1 !! c2 *)
+       split.
+       --- intros. remember (S i') as i.
+           destruct cont as [|h t] eqn:ELst.
+           ---- simpl. rewrite Heqi in H. simpl in H.
+                destruct (ceval_step st c1 i' []) as [(sst, si)| | ] eqn:Eceval.
+                ----- subst. apply IHi in Eceval. rewrite Eceval. 
+                      inversion H. trivial.
+                ----- apply IHi in H. rewrite H. 
+                      apply IHi in Eceval; trivial.
+                      rewrite Eceval. trivial.
+                ----- inversion H.
+           ---- simpl. rewrite Heqi in H. simpl in H.
+                destruct (ceval_step st c1 i' (h::t)) as [(sst, si)| | ] eqn:Eceval.
+                ----- subst. apply IHi in Eceval. rewrite Eceval. 
+                      inversion H. trivial.
+                ----- apply IHi in H. rewrite H. 
+                      apply IHi in Eceval; trivial.
+                      rewrite Eceval. trivial.
+                ----- inversion H.
+       --- intros. remember (S i') as i.
+           destruct cont as [|h t] eqn:ELst.
+           ---- simpl. rewrite Heqi in H. simpl in H.
+                destruct (ceval_step st c1 i' []) as [(sst, si)| | ] eqn:Eceval.
+                ----- subst. apply IHi in Eceval. rewrite Eceval. 
+                      inversion H.
+                ----- apply IHi in H; trivial. rewrite H. 
+                      apply IHi in Eceval; trivial.
+                      rewrite Eceval. trivial.
+                ----- inversion H.
+           ---- simpl. rewrite Heqi in H. simpl in H.
+                destruct (ceval_step st c1 i' (h::t)) as [(sst, si)| | ] eqn:Eceval.
+                ----- subst. apply IHi in Eceval. rewrite Eceval. 
+                      inversion H.
+                ----- apply IHi in H; trivial. rewrite H. 
+                      apply IHi in Eceval; trivial.
+                      rewrite Eceval. trivial.
+                ----- inversion H.
+    -- (* b -> c *)
+       split.
+       --- intros. remember (S i') as i.
+           destruct cont as [|h t] eqn:ELst.
+           ---- simpl. rewrite Heqi in H. simpl in H.
+                destruct (beval st b) eqn:Ebeval.
+                ----- apply IHi. trivial.
+                ----- inversion H.
+           ---- simpl. rewrite Heqi in H. simpl in H.
+                destruct (beval st b) eqn:Ebeval.
+                ----- apply IHi. trivial.
+                ----- inversion H.
+       --- intros. remember (S i') as i.
+           destruct cont as [|h t] eqn:ELst.
+           ---- simpl. rewrite Heqi in H. simpl in H.
+                destruct (beval st b) eqn:Ebeval.
+                ----- apply IHi; trivial.
+                ----- trivial.
+           ---- simpl. rewrite Heqi in H. simpl in H.
+                destruct (beval st b) eqn:Ebeval.
+                ----- apply IHi; trivial.
+                ----- trivial.
+(* only things admitted are the ones required for strong induction,
+   besides that everything was proven *)
+Admitted. 
+
+Lemma ceval_step_one_more: forall i f st st' c,
+  ceval_step_main st c i = Success (st', f) ->
+  ceval_step_main st c (S i) = Success (st', (S f)).
+Proof.
+  intros. unfold ceval_step_main. apply ceval_invariant. trivial.
+Qed.
+
+Theorem ceval_step_more: forall i1 i2 f1 st st' c ,
+  i1 <= i2 ->
+  ceval_step_main st c i1 = Success (st', f1) ->
+  exists f2, ceval_step_main st c i2 = Success (st', f2).
+Proof.
+  intros. exists (f1 + i2 - i1).
+  remember (f1 + (S i2) - i1) as f2.
+  remember (f2 - f1) as fdelta.
+  destruct fdelta as [|fdelta'] eqn:Edelta.
+  - assert (H': f1 = f2) by lia. 
+    assert (H'': i1 = i2) by lia.
+    rewrite H'.
+    rewrite <- H''.
+    lia. 
+  - assert (H': f2 = fdelta' + f1 + 1) by lia.
+    rewrite Heqf2 in H'.
+    assert (H'': i2 = fdelta' + i1) by lia.
+    rewrite H''.
+    subst.
+    induction fdelta' as [| fdelta'' IHdelta].
+    -- simpl. replace (f1 + i1 - i1) with f1.
+       --- assumption.
+       --- lia.
+    -- subst. replace (S fdelta'' + i1) with (S (i1 + fdelta'')); try lia.
+       replace (f1 + S (i1 + fdelta'') - i1) with (S( f1 + fdelta'')); try lia.
+       apply ceval_step_one_more.
+       assert (H'': f1 + S (fdelta'' + i1) - i1 = fdelta'' + f1 + 1 ) by lia.
+       apply IHdelta in H''; try lia.
+       replace (f1 + (fdelta'' + i1) - i1) with (f1 + fdelta'') in H''; try lia.
+       trivial. 
+       replace (i1 + fdelta'') with (fdelta'' + i1).
+       trivial.
+       lia.
+Qed.
+
+End CPS.
